verified/ARMprint.dfy
@@ -52,27 +52,55 @@ method printMode(m:mode)
         case Monitor => print("mon"); //TOOD check this
 }
 
+method printReg(r:ARMReg)
+{
+    match r
+        case R0 => print("r0");
+        case R1 => print("r1");
+        case R2 => print("r2");
+        case R3 => print("r3");
+        case R4 => print("r4");
+        case R5 => print("r5");
+        case R6 => print("r6");
+        case R7 => print("r7");
+        case R8 => print("r8");
+        case R9 => print("r9");
+        case R10 => print("r10");
+        case R11 => print("r11");
+        case R12 => print("r12");
+        case SP(m) => print("sp_"); printMode(m);
+        case LR(m) => print("lr_"); printMode(m);
+}
+
+method printShift(s:Shift)
+{
+    match s
+        case LSLShift(amount) => if amount == 0 { 
+                                     print("Shifts cannot be 0!"); 
+                                 } else { 
+                                     print("lsl#"); 
+                                     print(amount); 
+                                 }
+        case LSRShift(amount) => if amount == 0 { 
+                                     print("Shifts cannot be 0!"); 
+                                 } else { 
+                                     print("lsr#"); 
+                                     print(amount); 
+                                 }
+        case RORShift(amount) => if amount == 0 { 
+                                     print("Shifts cannot be 0!"); 
+                                 } else { 
+                                     print("ror#"); 
+                                     print(amount); 
+                                 }
+}
+
 method printOperand(o:operand)
 {
     match o
         case OConst(n) => print("#"); print(n);
-        case OReg(r) => {match r
-            case R0 => print("r0");
-            case R1 => print("r1");
-            case R2 => print("r2");
-            case R3 => print("r3");
-            case R4 => print("r4");
-            case R5 => print("r5");
-            case R6 => print("r6");
-            case R7 => print("r7");
-            case R8 => print("r8");
-            case R9 => print("r9");
-            case R10 => print("r10");
-            case R11 => print("r11");
-            case R12 => print("r12");
-            case SP(m) => print("sp_"); printMode(m);
-            case LR(m) => print("lr_"); printMode(m);
-        }
+        case OReg(r) => { printReg(r); }
+        case OShift(r, s) => { printReg(r); print(","); printShift(s); }
         case OSReg(r)   => {match r
            case ttbr0   => print("ttbr0");
            case scr     => print("scr");
